coq/Mono.v
@@ -1,23 +1,77 @@
-Require Import Coq.Strings.String.
-Require Import CoqRecon.Util.
+Require Import Coq.Strings.String CoqRecon.Util.
 
-Inductive type : Set :=
+Instance StringEqDec : EqDec string eq := {equiv_dec := string_dec}.
+
+Inductive typ : Set :=
 | TBool
 | TNat
-| TArrow : type -> type -> type
-| TVar : nat -> type.
+| TArrow : typ -> typ -> typ
+| TVar : nat -> typ.
+
+Declare Scope typ_scope.
+Delimit Scope typ_scope with typ.
+
+Notation "t1 → t2"
+  := (TArrow t1 t2)
+       (at level 30, right associativity) : typ_scope.
+
+Fixpoint tvars (t : typ) : list nat :=
+  match t with
+  | TBool | TNat => []
+  | TVar T => [T]
+  | (t → t')%typ => tvars t ++ tvars t'
+  end.
+
+Definition Ctvars : list (typ * typ) -> list nat :=
+  fold_right (fun '(l,r) acc => tvars l ++ tvars r ++ acc) [].
 
 Inductive op : Set :=
 | And | Or | Add | Sub | Eq | Lt.
 
 Inductive term : Set :=
 | Var : string -> term
-| Abs : string -> term
+| Abs : string -> term -> term
 | App : term -> term -> term
 | Bool : bool -> term
+| Nat : nat -> term
 | Cond : term -> term -> term
 | Op : op -> term -> term.
 
-Definition gamma : Set := @env string type.
+Declare Scope term_scope.
+Delimit Scope term_scope with term.
 
-Inductive typing (g : gamma) : term -> type -> list string -> Prop -> Prop :=.
+Notation "'λ' x ⇒ e"
+  := (Abs x e)
+       (at level 35, right associativity) : term_scope.
+Notation "e1 ⋅ e2"
+  := (App e1 e2)
+       (at level 34, left associativity) : term_scope.
+
+Definition gamma : Set := @env string typ.
+
+Reserved Notation "g ⊢ e ∈ t ⊣ X @ C" (at level 70).
+
+Inductive constraint_typing (Γ : gamma)
+  : term -> typ -> list nat -> list (typ * typ) -> Prop :=
+| ct_bool b :
+    Γ ⊢ Bool b ∈ TBool ⊣ [] @ []
+| ct_nat n :
+    Γ ⊢ Nat n ∈ TNat ⊣ [] @ []
+| ct_var x τ :
+    bound x τ Γ ->
+    Γ ⊢ Var x ∈ τ ⊣ [] @ []
+| ct_abs x e T τ X C :
+    ~ In T X ->
+    (x ↦ TVar T ;; Γ)%env ⊢ e ∈ τ ⊣ X @ C ->
+    Γ ⊢ (λ x ⇒ e)%term ∈ (TVar T → τ)%typ ⊣ (T :: X) @ C
+| ct_app e1 e2 T τ1 τ2 X1 X2 C1 C2 :
+    (X1 ∩ X2)%set = [] ->
+    (X1 ∩ tvars τ2)%set = [] ->
+    (X2 ∩ tvars τ1)%set = [] ->
+    ~ In T (X1 ++ X2 ++ tvars τ1 ++ tvars τ2 ++ Ctvars C1 ++ Ctvars C2) ->
+    Γ ⊢ e1 ∈ τ1 ⊣ X1 @ C1 ->
+    Γ ⊢ e2 ∈ τ2 ⊣ X2 @ C2 ->
+    Γ ⊢ (e1 ⋅ e2)%term ∈ TVar T
+      ⊣ (T :: X1 ++ X2) @ ((τ1, (τ2 → TVar T)%typ) :: C1 ++ C2)
+where "g ⊢ e ∈ t ⊣ X @ C"
+        := (constraint_typing g e t X C).
